src/program_proof/pav/client_hist.v
@@ -3,86 +3,171 @@ From Goose.github_com.mit_pdos.pav Require Import kt.
 
 From Perennial.program_proof.pav Require Import
   advrpc auditor core classes client cryptoffi evidence
-  logical_audit merkle msv rpc serde server.
+  logical_audit logical_hist merkle msv rpc serde server.
+
+Module hist_epochs_puts.
+
+(* length-extends hist with its last element. *)
+Definition lookup_epochs (hist : list $ option pk_ty) (ep : w64) :=
+  match hist !! (uint.nat ep) with
+  | Some opt_pk => opt_pk
+  | None => mjoin $ last hist
+  end.
+
+Definition reln epochs puts :=
+  ∀ ep,
+  lookup_epochs epochs ep = lookup_puts_hist puts ep.
+
+Lemma update_replicate epochs puts n :
+  reln epochs puts →
+  reln (epochs ++ replicate n (mjoin $ last epochs)) puts.
+Proof.
+  rewrite /reln /lookup_epochs.
+  intros Hreln ep.
+  ospecialize (Hreln ep).
+  rewrite last_replicate_option_app.
+  destruct (decide (uint.Z ep < Z.of_nat $ length epochs)).
+  { rewrite lookup_app_l; [done|word]. }
+  rewrite lookup_ge_None_2 in Hreln; [|word].
+  rewrite lookup_app_r; [|word].
+  case_match; [|done].
+  apply lookup_replicate in H.
+  intuition.
+  by simplify_eq/=.
+Qed.
+
+Lemma update_new epochs puts ep pk :
+  (* something to tie together epochs and puts (ep). *)
+  Z.of_nat $ length epochs = uint.Z ep →
+  reln epochs puts →
+  reln (epochs ++ [Some pk]) (puts ++ [(ep, pk)]).
+Proof.
+  rewrite /reln /lookup_epochs /lookup_puts_hist.
+  intros ? Hreln ep0.
+  rewrite filter_snoc /=.
+  destruct (decide (uint.Z ep0 < Z.of_nat $ length epochs)).
+  (* revert lookups back to the original hists. *)
+  - ospecialize (Hreln ep0).
+    (* epochs. *)
+    rewrite lookup_app_l; [|word].
+    opose proof (list_lookup_lt epochs (uint.nat ep0) _) as [? Ht]; [word|].
+    rewrite Ht in Hreln |-*.
+    (* puts. *)
+    case_decide; [word|].
+    by list_simplifier.
+  (* extract snoc'd entry out of hists. *)
+  - clear Hreln.
+    (* puts. *)
+    case_decide; [|word].
+    rewrite !last_snoc /=.
+    (* epochs. *)
+    rewrite lookup_app_r; [|word].
+    case_match; [|done].
+    by list_simplifier.
+Qed.
+
+End hist_epochs_puts.
+
+Module ClientHist.
+Record t :=
+  mk {
+    γ: gname;
+    uid: w64;
+    (* epochs_hist allows stating the "intuitive" KT consistency property:
+    that a client knows its key at every epoch. *)
+    epochs_hist: list (option pk_ty);
+    serv: Server.t;
+    serv_is_good: bool;
+  }.
+Global Instance eta : Settable _ :=
+  settable! mk <γ; uid; epochs_hist; serv; serv_is_good>.
+
+Section defs.
+Context `{!heapGS Σ, !pavG Σ}.
+
+Definition own (ptr : loc) (obj : t) : iProp Σ :=
+  ∃ puts_hist (next_epoch : w64),
+  (* this doesn't hold for Get ops, but those are intentionally not part
+  of the ClientHist api. *)
+  "%Heq_next_ep" ∷ ⌜ Z.of_nat $ length obj.(epochs_hist) = uint.Z next_epoch ⌝ ∗
+  "%Hhist_reln" ∷ ⌜ hist_epochs_puts.reln obj.(epochs_hist) puts_hist ⌝ ∗
+
+  "Hcli" ∷ Client.own ptr (Client.mk obj.(γ) obj.(uid)
+    (W64 $ length puts_hist) next_epoch obj.(serv) obj.(serv_is_good)) ∗
+  "#Hhist" ∷ is_hist obj.(γ) obj.(serv).(Server.vrf_pk) obj.(uid)
+    puts_hist next_epoch.
+
+Lemma lookup_msv ptr_c c ep opt_pk γaudit aud_ep :
+  c.(epochs_hist) !! (uint.nat ep) = Some opt_pk →
+  (* it's hard to give tighter aud_ep bound, since a particular ep of
+  epochs_hist might only be an msv with some later ep bound. *)
+  Z.of_nat $ length c.(epochs_hist) <= uint.Z aud_ep →
+  own ptr_c c -∗
+  logical_audit c.(γ) γaudit c.(serv).(Server.vrf_pk) aud_ep -∗
+  msv γaudit c.(serv).(Server.vrf_pk) ep c.(uid) opt_pk.
+Proof.
+  iIntros (Hlook ?) "H #Haudit". iNamed "H".
+  ospecialize (Hhist_reln ep).
+  rewrite /hist_epochs_puts.lookup_epochs Hlook in Hhist_reln.
+  subst.
+  iDestruct (hist_to_msv ep with "Hhist Haudit") as "$".
+  { apply lookup_lt_Some in Hlook. word. }
+  { word. }
+Qed.
+
+End defs.
+End ClientHist.
 
 Section proof.
 Context `{!heapGS Σ, !pavG Σ}.
 
-Definition is_hist c γaudit hist : iProp Σ :=
-  "%Hnil_hist" ∷ ⌜ hist = [] → c.(Client.next_ver) = (W64 0) ⌝ ∗
-  "%Hhist_len" ∷ ⌜ Z.of_nat (length hist) = uint.Z c.(Client.next_epoch) ⌝ ∗
-  (* for all epochs, msv. *)
-  "#Hall_hist" ∷ (∀ ep opt_pk,
-    ⌜ hist !! (uint.nat ep) = Some opt_pk ⌝ -∗
-    msv γaudit c.(Client.serv).(Server.vrf_pk) ep c.(Client.uid) opt_pk) ∗
-  (* for last epoch, msv with associated n_vers. *)
-  "#Hlast_hist" ∷ (∀ opt_pk,
-    ⌜ last hist = Some opt_pk ⌝ -∗
-    msv_vers γaudit c.(Client.serv).(Server.vrf_pk)
-      (W64 (length hist - 1)) c.(Client.uid) opt_pk c.(Client.next_ver)).
-
 Lemma wp_ClientHist__Put ptr_c c sl_pk d0 (pk : list w8) :
   {{{
-    "Hcli" ∷ Client.own ptr_c c ∗
+    "Hcli" ∷ ClientHist.own ptr_c c ∗
     "Hsl_pk" ∷ own_slice_small sl_pk byteT d0 pk
   }}}
   Client__Put #ptr_c (slice_val sl_pk)
   {{{
-    err (bound_ep : w64) ptr_err, RET (#bound_ep, #ptr_err);
+    err (ep : w64) ptr_err, RET (#ep, #ptr_err);
     "Hsl_pk" ∷ own_slice_small sl_pk byteT d0 pk ∗
-    "Hown_err" ∷ ClientErr.own ptr_err err c.(Client.serv).(Server.sig_pk) ∗
-    "%Hgenie" ∷ ⌜ c.(Client.serv_is_good) = true → err.(ClientErr.Err) = false ⌝ ∗
+    "Hown_err" ∷ ClientErr.own ptr_err err c.(ClientHist.serv).(Server.sig_pk) ∗
+    "%Hgenie" ∷ ⌜ c.(ClientHist.serv_is_good) = true → err.(ClientErr.Err) = false ⌝ ∗
 
     "Herr" ∷ (if err.(ClientErr.Err)
       then
-        "Hcli" ∷ Client.own ptr_c c
+        "Hcli" ∷ ClientHist.own ptr_c c
       else
-        ∃ next_ver next_ep,
-        let new_c := set Client.next_ver (λ _, next_ver)
-          (set Client.next_epoch (λ _, next_ep) c) in
-        "Hcli" ∷ Client.own ptr_c new_c ∗
-
-        "#Hhist_updater" ∷ (□ ∀ γaudit audit_ep,
-          ⌜ uint.Z next_ep <= uint.Z audit_ep ⌝ -∗
-          logical_audit c.(Client.γ) γaudit c.(Client.serv).(Server.vrf_pk) audit_ep -∗
-
-          (* can't put old_hist in precond.
-          it'd be under existential (see below),
-          so we couldn't reference / extend it in new_hist.
-          instead, need this "updater"-style, which is more clunky to use. *)
-          ∀ old_hist,
-          is_hist c γaudit old_hist -∗
-
-          (* ∃ insert_ep must come after logical_audit bc it's derived
-          from the auditor's monotonicity invariant. *)
-          ∃ (insert_ep : w64),
-          let last_len := uint.Z insert_ep - Z.of_nat (length old_hist) in
-          let new_len := uint.Z bound_ep - uint.Z insert_ep + 1 in
-          let new_hist := old_hist ++
-            replicate (Z.to_nat last_len) (mjoin $ last old_hist) ++
-            replicate (Z.to_nat new_len) (Some pk) in
-          ⌜ Z.of_nat (length old_hist) <= uint.Z insert_ep <= uint.Z bound_ep ⌝ ∗
-          ⌜ uint.Z $ word.add bound_ep (W64 1) = (uint.Z bound_ep + 1)%Z ⌝ ∗
-          is_hist new_c γaudit new_hist))
+        let len_diff := uint.Z ep - Z.of_nat (length c.(ClientHist.epochs_hist)) in
+        let new_c := set ClientHist.epochs_hist (λ x, x ++
+          replicate (Z.to_nat len_diff) (mjoin $ last x) ++
+          [Some pk]) c in
+        "%Hlt_diff" ∷ ⌜ len_diff >= 0 ⌝ ∗
+        "%Hnoof_ep" ∷ ⌜ uint.Z $ word.add ep (W64 1) = (uint.Z ep + 1)%Z ⌝ ∗
+        "Hcli" ∷ ClientHist.own ptr_c new_c)
   }}}.
 Proof.
-  iIntros (Φ) "H HΦ". iNamed "H".
-  destruct c. simpl.
+  iIntros (Φ) "H HΦ". iNamed "H". iNamed "Hcli".
+  destruct c. simpl in *.
   wp_apply (wp_Client__Put with "[$Hcli $Hsl_pk]").
   simpl. iIntros "*". iNamed 1.
   iApply "HΦ". iFrame "∗%".
   case_match; iNamed "Herr"; [by iFrame "∗#"|].
-  iFrame.
-
-  iIntros "!> * % #Haudit *".
-  iNamedSuffix 1 "_old". simpl in *.
-  destruct (last old_hist) eqn:Heq_last.
-  2: {
-    iClear "Hall_hist_old Hlast_hist_old".
-    apply last_None in Heq_last as ->.
-    opose proof (Hnil_hist_old _) as ->; [done|].
-    iNamed "Haudit".
-Admitted.
+  iSplit; [word|].
+  iSplit; [word|].
+  iExists (puts_hist ++ [(ep, pk)]), (word.add ep (W64 1)).
+  do 3 try iSplit; simpl in *.
+  - rewrite !length_app length_replicate /=. word.
+  - iPureIntro.
+    rewrite (assoc (++)).
+    apply hist_epochs_puts.update_new.
+    { rewrite length_app length_replicate. word. }
+    by apply hist_epochs_puts.update_replicate.
+  - rewrite length_app /=.
+    replace (W64 (_ + _)%nat) with
+      (word.add (W64 $ length puts_hist) (W64 1)); [|word].
+    iFrame.
+  - iApply (hist_extend_put with "[$Hhist $His_put_post]"); word.
+Qed.
 
 Lemma wp_ClientHist__SelfMon ptr_c c :
   {{{
