src/program_proof/pav/core.v
@@ -2,22 +2,28 @@ From Perennial.program_proof.pav Require Import prelude.
 
 From Perennial.program_proof.pav Require Import cryptoffi serde.
 
-(* data at two different levels of opaqueness might both be (list w8)'s.
-these notations provide a reference for their logical meaning. *)
+(* TODO: for same reason not using alias's in go code,
+prob shouldn't define all these notations. *)
+Notation commit_ty := (list w8) (only parsing).
+Notation dig_ty := (list w8) (only parsing).
 Notation uid_ty := w64 (only parsing).
 Notation ver_ty := w64 (only parsing).
-Notation map_label_ty := (uid_ty * ver_ty)%type (only parsing).
-Notation opaq_label_ty := (list w8) (only parsing).
-Notation pk_ty := (list w8) (only parsing).
-Notation commit_ty := (list w8) (only parsing).
-Notation map_val_ty := (pk_ty) (only parsing).
-Notation opaq_val_ty := (commit_ty) (only parsing).
-
 Notation epoch_ty := w64 (only parsing).
-Notation dig_ty := (list w8) (only parsing).
-Notation merkle_map_ty := (gmap opaq_label_ty opaq_val_ty) (only parsing).
+Notation pk_ty := (list w8) (only parsing).
+Notation map_label_ty := (uid_ty * ver_ty)%type (only parsing).
+Notation opaque_label_ty := (list w8) (only parsing).
+Notation map_val_ty := (epoch_ty * pk_ty)%type (only parsing).
+Notation map_ty := (gmap map_label_ty map_val_ty) (only parsing).
+Notation merkle_map_ty := (gmap (list w8) (list w8)) (only parsing).
+Notation opaque_map_val_ty := (epoch_ty * commit_ty)%type (only parsing).
+Notation adtr_map_ty := (gmap opaque_label_ty opaque_map_val_ty) (only parsing).
+Notation cli_map_val_ty := (option (epoch_ty * commit_ty)) (only parsing).
+Notation cli_map_ty := (gmap map_label_ty cli_map_val_ty) (only parsing).
+Notation lat_val_ty := (option map_val_ty) (only parsing).
+Notation lat_opaque_val_ty := (option opaque_map_val_ty) (only parsing).
 
 Notation enc_label_pre uid ver := (MapLabelPre.encodesF $ MapLabelPre.mk uid ver).
+Notation enc_val ep commit := (MapValPre.encodesF $ MapValPre.mk ep commit).
 Notation enc_sigdig ep dig := (PreSigDig.encodesF $ PreSigDig.mk ep dig).
 
 Section defs.
@@ -25,15 +31,18 @@ Section defs.
 Class pavG Σ :=
   {
     #[global] pavG_serv_ep :: mono_natG Σ;
-    #[global] pavG_serv_vers :: ghost_mapG Σ uid_ty ver_ty;
-    #[global] pavG_adtr :: mono_listG (merkle_map_ty * dig_ty) Σ;
+    #[global] pavG_serv_digs ::
+      mono_listG ((gmap (list w8) (w64 * list w8)) * list w8) Σ;
+    #[global] pavG_serv_map :: ghost_mapG Σ w64 w64;
+    #[global] pavG_adtr ::
+      mono_listG ((gmap opaque_label_ty (epoch_ty * commit_ty)) * dig_ty) Σ;
     #[global] pavG_cli :: mono_listG (option dig_ty) Σ;
   }.
 
 Context `{!heapGS Σ}.
 
 Definition is_map_label pk uid ver label : iProp Σ :=
-  is_vrf_out pk (enc_label_pre uid ver) label.
+  is_vrf_out pk (MapLabelPre.encodesF $ MapLabelPre.mk uid ver) label.
 
 Definition is_commit (val : pk_ty) (commit : commit_ty) : iProp Σ :=
   ∃ rand enc,
@@ -48,5 +57,8 @@ Proof.
   opose proof (CommitOpen.inj [] [] Henc0 Henc1 _) as ?; [done|].
   naive_solver.
 Qed.
+
+Definition lookup_puts_hist (hist : list map_val_ty) (ep : w64) :=
+  snd <$> (last $ filter (λ x, uint.Z x.1 ≤ uint.Z ep) hist).
 
 End defs.
