src/program_proof/pav/logical_audit.v
@@ -4,70 +4,31 @@ From Perennial.program_proof.pav Require Import core serde merkle.
 Section proof.
 Context `{!heapGS Σ, !pavG Σ}.
 
-Definition mono_maps (ms : list merkle_map_ty) :=
+Definition mono_maps (ms : list adtr_map_ty) :=
   ∀ (i j : w64) mi mj,
   ms !! (uint.nat i) = Some mi →
   ms !! (uint.nat j) = Some mj →
   uint.Z i ≤ uint.Z j →
   mi ⊆ mj.
 
-(* our "characterization" of monotonic maps. *)
-Lemma mono_char ms :
-  mono_maps ms →
-  ∀ k,
-  (* all flat. *)
-  (∀ (ep : w64) m_ep,
-    ms !! (uint.nat ep) = Some m_ep →
-    m_ep !! k = None)
-  ∨
-  (∃ (insert_ep : w64) m_insert,
-    (* flat. *)
-    (∀ (ep : w64),
-      uint.Z ep < uint.Z insert_ep →
-      ∃ m_ep,
-      ms !! (uint.nat ep) = Some m_ep ∧
-      m_ep !! k = None) ∧
-    (* until a spike. *)
-    ms !! (uint.nat insert_ep) = Some m_insert ∧
-    is_Some (m_insert !! k)).
-Proof. Admitted.
+Definition ok_epochs (ms : list adtr_map_ty) :=
+  ∀ (ep : w64) m_ep k ep' comm,
+  ms !! (uint.nat ep) = Some m_ep →
+  m_ep !! k = Some (ep', comm) →
+  uint.Z ep' ≤ uint.Z ep.
 
-Lemma mono_get_insertion ms (bound_ep : w64) m_bound k :
-  mono_maps ms →
-  ms !! (uint.nat bound_ep) = Some m_bound →
-  is_Some (m_bound !! k) →
+(* TODO: maybe change adtr_map_ty to have MapValPre instead of pair. *)
+Definition map_lower (higher : adtr_map_ty) (lower : merkle_map_ty) :=
+  map_Forall2 (λ _ x y, MapValPre.encodes x y) lower
+    ((λ x, MapValPre.mk x.1 x.2) <$> higher).
 
-  ∃ (insert_ep : w64) m_insert,
-  ms !! (uint.nat insert_ep) = Some m_insert ∧
-  is_Some (m_insert !! k) ∧
-  (
-    uint.Z insert_ep = 0
-    ∨
-    ∀ m_pred,
-    ms !! (Z.to_nat (uint.Z insert_ep - 1)) = Some m_pred →
-    m_pred !! k = None
-  ).
-Proof.
-  intros Hmono Hlook_end ?.
-  opose proof (mono_char _ Hmono k) as [Hmono1 | Hmono1].
-  - exfalso. ospecialize (Hmono1 _ _ Hlook_end).
-    destruct (m_bound !! k); [done|].
-    by eapply is_Some_None.
-  - destruct Hmono1 as (insert_ep&?&Hflat&Hlook_insert&?).
-    eexists insert_ep, _.
-    repeat try split; [done..|].
-    destruct (decide (uint.Z insert_ep = 0)); [naive_solver|].
-    right. intros ? Hlook_pred0.
-    remember (word.sub insert_ep (W64 1)) as i.
-    replace (Z.to_nat _) with (uint.nat i) in Hlook_pred0 by word.
-    opose proof (Hflat i _) as (?&Hlook_pred1&?); [word|].
-    by simplify_eq/=.
-Qed.
-
-Definition audit_gs_inv (gs : list (merkle_map_ty * dig_ty)) : iProp Σ :=
+Definition audit_gs_inv (gs : list (adtr_map_ty * dig_ty)) : iProp Σ :=
   "#His_digs" ∷ ([∗ list] x ∈ gs,
-    "#His_map" ∷ is_merkle_map x.1 x.2) ∗
-  "%Hmono_maps" ∷ ⌜ mono_maps gs.*1 ⌝.
+    ∃ lower,
+    "%Hlower" ∷ ⌜ map_lower x.1 lower ⌝ ∗
+    "#His_map" ∷ is_merkle_map lower x.2) ∗
+  "%Hmono_maps" ∷ ⌜ mono_maps gs.*1 ⌝ ∗
+  "%Hok_epochs" ∷ ⌜ ok_epochs gs.*1 ⌝.
 
 Definition sigpred γ : (list w8 → iProp Σ) :=
   λ preByt,
@@ -77,18 +38,20 @@ Definition sigpred γ : (list w8 → iProp Σ) :=
   "%Hlook_dig" ∷ ⌜ gs !! uint.nat pre.(PreSigDig.Epoch) = Some (m, pre.(PreSigDig.Dig)) ⌝ ∗
   "#Hinv_gs" ∷ audit_gs_inv gs)%I.
 
-Lemma audit_gs_snoc gs upd dig :
+Lemma audit_gs_snoc gs upd lowered_new_map dig :
   let new_map := (upd ∪ (default ∅ (last gs.*1))) in
   upd ##ₘ (default ∅ (last gs.*1)) →
+  map_lower new_map lowered_new_map →
+  map_Forall (λ _ v, v.1 = W64 (length gs)) upd →
   audit_gs_inv gs -∗
-  is_merkle_map new_map dig -∗
+  is_merkle_map lowered_new_map dig -∗
   audit_gs_inv (gs ++ [(new_map, dig)]).
 Proof.
-  simpl. iIntros (Hdisj) "#Hold_inv #His_dig".
+  simpl. iIntros (Hdisj Hlower Hok_epoch) "#Hold_inv #His_dig".
   iNamedSuffix "Hold_inv" "_old".
-  iSplit.
+  iSplit; [|iPureIntro; split].
   - iApply big_sepL_snoc. iFrame "#%".
-  - iPureIntro. unfold mono_maps in *. intros * Hlook_gsi Hlook_gsj Heq_ep.
+  - unfold mono_maps in *. intros * Hlook_gsi Hlook_gsj Heq_ep.
     rewrite fmap_app in Hlook_gsi Hlook_gsj.
     destruct (decide (uint.Z i = uint.Z j)).
     { by simplify_eq/=. }
@@ -114,6 +77,23 @@ Proof.
       (W64 (pred $ length gs)) _ _ Hlook_gsi _ _); [|word].
     replace (uint.nat (W64 _)) with (pred $ length gs); [|word].
     by rewrite length_fmap in Hlast.
+  - unfold ok_epochs in *. intros * Hlook_gs Hlook_m.
+    rewrite fmap_app in Hlook_gs.
+    destruct (decide (uint.Z ep < length gs)).
+    { eapply Hok_epochs_old; [|done].
+      rewrite lookup_app_l in Hlook_gs; [done|].
+      rewrite length_fmap. word. }
+    rewrite lookup_app_r in Hlook_gs.
+    2: { rewrite length_fmap. word. }
+    simpl in *. apply list_lookup_singleton_Some in Hlook_gs as [Heq_ep <-].
+    apply lookup_union_Some_raw in Hlook_m as [Hlook_upd | [_ Hlook_last]].
+    { pose proof (map_Forall_lookup_1 _ _ _ _ Hok_epoch Hlook_upd) as ?.
+      simpl in *. subst. word. }
+    destruct (last gs.*1) as [m_last|] eqn:Hlast; [|set_solver]. simpl in *.
+    opose proof (Hok_epochs_old
+      (W64 (pred $ length gs)) _ _ _ _ _ Hlook_last) as ?; [|word].
+    replace (uint.nat (W64 _)) with (pred $ length gs); [|word].
+    by rewrite last_lookup length_fmap in Hlast.
 Qed.
 
 Lemma audit_gs_prefix l l' :
@@ -121,14 +101,18 @@ Lemma audit_gs_prefix l l' :
   audit_gs_inv l -∗
   audit_gs_inv l'.
 Proof.
-  iIntros (Hpref). iNamed 1. iSplit.
+  iIntros (Hpref). iNamed 1. iSplit; [|iPureIntro; split].
   - opose proof (prefix_to_take _ _ Hpref) as ->.
     by iApply big_sepL_take.
-  - iPureIntro. intros ???? Hlook0 Hlook1 ?.
+  - intros ???? Hlook0 Hlook1 ?.
     apply (prefix_fmap fst) in Hpref.
     opose proof (prefix_lookup_Some _ _ _ _ Hlook0 Hpref) as Hlook0'.
     opose proof (prefix_lookup_Some _ _ _ _ Hlook1 Hpref) as Hlook1'.
     by apply (Hmono_maps _ _ _ _ Hlook0' Hlook1').
+  - intros ????? Hlook0 Hlook1.
+    apply (prefix_fmap fst) in Hpref.
+    opose proof (prefix_lookup_Some _ _ _ _ Hlook0 Hpref) as Hlook0'.
+    by apply (Hok_epochs _ _ _ _ _ Hlook0' Hlook1).
 Qed.
 
 End proof.
