src/program_proof/pav/msv.v
@@ -16,17 +16,17 @@ this difference is why we separated the "history" and "latest" resources. *)
 Section proof.
 Context `{!heapGS Σ, !pavG Σ}.
 
-Definition msv_Some (m : merkle_map_ty) vrf_pk uid pk n_vers : iProp Σ :=
+Definition msv_Some (m : adtr_map_ty) vrf_pk uid pk n_vers : iProp Σ :=
   "#Hhist" ∷
     (∀ ver, ⌜ uint.Z ver < uint.Z (word.sub n_vers (W64 1)) ⌝ -∗
     ∃ label val,
     "#Hlabel" ∷ is_map_label vrf_pk uid ver label ∗
     "%Hlook_map" ∷ ⌜ m !! label = Some val ⌝) ∗
   "#Hlatest" ∷
-    (∃ commit label,
+    (∃ ep commit label,
     "#Hcommit" ∷ is_commit pk commit ∗
     "#Hlabel" ∷ is_map_label vrf_pk uid (word.sub n_vers (W64 1)) label ∗
-    "%Hlook_map" ∷ ⌜ m !! label = Some commit ⌝) ∗
+    "%Hlook_map" ∷ ⌜ m !! label = Some (ep, commit) ⌝) ∗
   "#Hbound" ∷
     (∃ label,
     "#Hlabel" ∷ is_map_label vrf_pk uid n_vers label ∗
@@ -78,7 +78,7 @@ Proof.
   naive_solver.
 Qed.
 
-Definition msv_None (m : merkle_map_ty) vrf_pk uid : iProp Σ :=
+Definition msv_None (m : adtr_map_ty) vrf_pk uid : iProp Σ :=
   ∃ label,
   "#Hlabel" ∷ is_map_label vrf_pk uid (W64 0) label ∗
   "%Hlook_map" ∷ ⌜ m !! label = None ⌝.
@@ -102,38 +102,25 @@ Proof.
     naive_solver.
 Qed.
 
-(* expose n_vers since it's needed to match up to physical code. *)
-Definition msv_vers γaudit vrf_pk (ep : w64) uid opt_pk n_vers : iProp Σ :=
+Definition msv γaudit vrf_pk (ep : w64) uid opt_pk : iProp Σ :=
   ∃ m dig,
   "#Hlook_gs" ∷ mono_list_idx_own γaudit (uint.nat ep) (m, dig) ∗
   "#Hmsv" ∷ match opt_pk with
-    | None =>
-      "%Heq_vers" ∷ ⌜ uint.Z n_vers = 0 ⌝ ∗
-      "#Hmsv" ∷ msv_None m vrf_pk uid
-    | Some pk => "#Hmsv" ∷ msv_Some m vrf_pk uid pk n_vers
+    | None => "#Hmsv" ∷ msv_None m vrf_pk uid
+    | Some pk => ∃ n_vers, "#Hmsv" ∷ msv_Some m vrf_pk uid pk n_vers
     end.
-
-Definition msv γaudit vrf_pk (ep : w64) uid opt_pk : iProp Σ :=
-  match opt_pk with
-  | None => "#Hmsv" ∷ msv_vers γaudit vrf_pk ep uid None (W64 0)
-  | Some pk => ∃ n_vers, "#Hmsv" ∷ msv_vers γaudit vrf_pk ep uid (Some pk) n_vers
-  end.
 
 Lemma msv_agree γ vrf_pk ep uid opt_pk0 opt_pk1 :
   msv γ vrf_pk ep uid opt_pk0 -∗
   msv γ vrf_pk ep uid opt_pk1 -∗
   ⌜ opt_pk0 = opt_pk1 ⌝.
 Proof.
-  destruct opt_pk0, opt_pk1; simpl;
-    iNamedSuffix 1 "0"; iNamedSuffix 1 "1";
-    iNamedSuffix "Hmsv0" "0"; iNamedSuffix "Hmsv1" "1";
-    iNamedSuffix "Hmsv0" "0"; iNamedSuffix "Hmsv1" "1";
-    [..|done].
-  (* TODO: mono_list_idx_agree not working in tactic chain bc of some weird
-  unification issues with the list elems being pairs. *)
-  - iDestruct (mono_list_idx_agree with "Hlook_gs0 Hlook_gs1") as %?.
-    simplify_eq/=.
-    iDestruct (msv_Some_vers_agree with "Hmsv0 Hmsv1") as %->.
+  iNamedSuffix 1 "0". iNamedSuffix 1 "1".
+  iDestruct (mono_list_idx_agree with "Hlook_gs0 Hlook_gs1") as %?.
+  simplify_eq/=.
+  destruct opt_pk0, opt_pk1; [..|done];
+    iNamedSuffix "Hmsv0" "0"; iNamedSuffix "Hmsv1" "1".
+  - iDestruct (msv_Some_vers_agree with "Hmsv0 Hmsv1") as %->.
     iNamedSuffix "Hmsv0" "0". iNamedSuffix "Hmsv1" "1".
     iClear "Hhist0 Hbound0 Hhist1 Hbound1".
     iNamedSuffix "Hlatest0" "0". iNamedSuffix "Hlatest1" "1".
@@ -141,12 +128,8 @@ Proof.
     simplify_eq/=.
     iDestruct (is_commit_inj with "Hcommit0 Hcommit1") as %?.
     by simplify_eq/=.
-  - iDestruct (mono_list_idx_agree with "Hlook_gs0 Hlook_gs1") as %?.
-    simplify_eq/=.
-    iDestruct (msv_Some_None_excl with "Hmsv0 Hmsv1") as "[]".
-  - iDestruct (mono_list_idx_agree with "Hlook_gs0 Hlook_gs1") as %?.
-    simplify_eq/=.
-    iDestruct (msv_Some_None_excl with "Hmsv1 Hmsv0") as "[]".
+  - iDestruct (msv_Some_None_excl with "Hmsv0 Hmsv1") as "[]".
+  - iDestruct (msv_Some_None_excl with "Hmsv1 Hmsv0") as "[]".
 Qed.
 
 End proof.
