external/Goose/github_com/mit_pdos/pav/alicebob.v
@@ -79,27 +79,44 @@ Definition checkCliErr: val :=
       control.impl.Assume (~ (struct.loadF kt.ClientErr "Err" "err"));;
       #()).
 
+(* histEntry from history.go *)
+
 Definition histEntry := struct.decl [
   "isReg" :: boolT;
   "pk" :: slice.T byteT
 ].
 
+(* extendHist to length numEpochs.
+   numEpochs must not be smaller than length hist. *)
+Definition extendHist: val :=
+  rec: "extendHist" "hist" "numEpochs" :=
+    let: "histLen" := slice.len "hist" in
+    std.Assert ("histLen" ≤ "numEpochs");;
+    let: "last" := ref (zero_val ptrT) in
+    (if: "histLen" = #0
+    then
+      "last" <-[ptrT] (struct.new histEntry [
+      ])
+    else "last" <-[ptrT] (SliceGet ptrT "hist" ("histLen" - #1)));;
+    let: "newHist" := ref_to (slice.T ptrT) "hist" in
+    let: "i" := ref_to uint64T "histLen" in
+    Skip;;
+    (for: (λ: <>, (![uint64T] "i") < "numEpochs"); (λ: <>, "i" <-[uint64T] ((![uint64T] "i") + #1)) := λ: <>,
+      "newHist" <-[slice.T ptrT] (SliceAppend ptrT (![slice.T ptrT] "newHist") (![ptrT] "last"));;
+      Continue);;
+    ![slice.T ptrT] "newHist".
+
+(* alice__run from alicebob.go *)
+
 Definition alice__run: val :=
   rec: "alice__run" "a" :=
-    let: ("startEp", "err0") := kt.Client__SelfMon (struct.loadF alice "cli" "a") in
-    checkCliErr (struct.loadF alice "servGood" "a") (struct.loadF alice "servSigPk" "a") "err0";;
-    control.impl.Assume ("startEp" = #0);;
-    struct.storeF alice "hist" "a" (SliceAppend ptrT (struct.loadF alice "hist" "a") (struct.new histEntry [
-      "isReg" ::= #false
-    ]));;
-    time.Sleep #5000000;;
     let: "i" := ref_to uint64T #0 in
     (for: (λ: <>, (![uint64T] "i") < #20); (λ: <>, "i" <-[uint64T] ((![uint64T] "i") + #1)) := λ: <>,
       time.Sleep #5000000;;
       let: "pk" := SliceSingleton #(U8 1) in
-      let: ("putEpoch", "err1") := kt.Client__Put (struct.loadF alice "cli" "a") "pk" in
-      checkCliErr (struct.loadF alice "servGood" "a") (struct.loadF alice "servSigPk" "a") "err1";;
-      control.impl.Assume ("putEpoch" = (slice.len (struct.loadF alice "hist" "a")));;
+      let: ("epoch", "err0") := kt.Client__Put (struct.loadF alice "cli" "a") "pk" in
+      checkCliErr (struct.loadF alice "servGood" "a") (struct.loadF alice "servSigPk" "a") "err0";;
+      struct.storeF alice "hist" "a" (extendHist (struct.loadF alice "hist" "a") "epoch");;
       struct.storeF alice "hist" "a" (SliceAppend ptrT (struct.loadF alice "hist" "a") (struct.new histEntry [
         "isReg" ::= #true;
         "pk" ::= "pk"
@@ -186,13 +203,16 @@ Definition testAliceBob: val :=
     Fork (bob__run "bob";;
           waitgroup.Done "wg");;
     waitgroup.Wait "wg";;
+    let: ("selfMonEp", "err0") := kt.Client__SelfMon (struct.loadF alice "cli" "alice") in
+    checkCliErr (struct.loadF setupParams "servGood" "setup") (struct.loadF setupParams "servSigPk" "setup") "err0";;
+    struct.storeF alice "hist" "alice" (extendHist (struct.loadF alice "hist" "alice") ("selfMonEp" + #1));;
     (if: struct.loadF setupParams "adtrGood" "setup"
     then
       updAdtrsAll (struct.loadF setupParams "servAddr" "setup") (struct.loadF setupParams "adtrAddrs" "setup");;
       doAudits (struct.loadF alice "cli" "alice") (struct.loadF setupParams "adtrAddrs" "setup") (struct.loadF setupParams "adtrPks" "setup");;
       doAudits (struct.loadF bob "cli" "bob") (struct.loadF setupParams "adtrAddrs" "setup") (struct.loadF setupParams "adtrPks" "setup")
     else #());;
-    control.impl.Assume ((struct.loadF bob "epoch" "bob") < (slice.len (struct.loadF alice "hist" "alice")));;
+    control.impl.Assume ((struct.loadF bob "epoch" "bob") ≤ "selfMonEp");;
     let: "aliceKey" := SliceGet ptrT (struct.loadF alice "hist" "alice") (struct.loadF bob "epoch" "bob") in
     std.Assert ((struct.loadF histEntry "isReg" "aliceKey") = (struct.loadF bob "isReg" "bob"));;
     (if: struct.loadF histEntry "isReg" "aliceKey"
@@ -222,5 +242,7 @@ Definition testCorrectness: val :=
     #().
 
 (* helpers.go *)
+
+(* history.go *)
 
 End code.
